finished SC-level verification proof

intermediate/Veritas.Intermediate.Logs.fst
@@ -4,59 +4,40 @@ open Veritas.Key
 open Veritas.MultiSetHashDomain
 open Veritas.Record
 open Veritas.SeqAux
-open Veritas.Intermediate.StoreSKC
 
 module Spec = Veritas.Verifier
 
+let slot_id = nat
 let thread_id = Spec.thread_id
 
 (* Definitions of different styles of verifier logs.
    - logK : contains only key references (defined in Veritas.Verifier)
-   - logSK: contains both slot and key references
-   - logS: contains only slot references *)
+   - logS: contains slot references
+   - logL: contains slot references & low-level data structures (TODO) *)
 
 let logK_entry = Spec.vlog_entry
 let logK = Spec.vlog
 
-noeq
-type logSK_entry =
-  | Get_SK: s:slot_id -> k:data_key -> v:data_value -> logSK_entry
-  | Put_SK: s:slot_id -> k:data_key -> v:data_value -> logSK_entry
-  | AddM_SK: s:slot_id -> r:record -> s':slot_id -> k':merkle_key -> logSK_entry
-  | EvictM_SK: s:slot_id -> k:key -> s':slot_id -> k':merkle_key -> logSK_entry
-  | AddB_SK: s:slot_id -> r:record -> t:timestamp -> j:thread_id -> logSK_entry
-  | EvictB_SK: s:slot_id -> k:key -> t:timestamp -> logSK_entry
-  | EvictBM_SK: s:slot_id -> k:key -> s':slot_id -> k':merkle_key -> t:timestamp -> logSK_entry
-             
-let logSK = Seq.seq logSK_entry
-
-noeq
 type logS_entry =
-  | Get_S: s:slot_id -> v:data_value -> logS_entry
-  | Put_S: s:slot_id -> v:data_value -> logS_entry
+  | Get_S: s:slot_id -> k:data_key -> v:data_value -> logS_entry
+  | Put_S: s:slot_id -> k:data_key -> v:data_value -> logS_entry
   | AddM_S: s:slot_id -> r:record -> s':slot_id -> logS_entry
   | EvictM_S: s:slot_id -> s':slot_id -> logS_entry
   | AddB_S: s:slot_id -> r:record -> t:timestamp -> j:thread_id -> logS_entry
   | EvictB_S: s:slot_id -> t:timestamp -> logS_entry
   | EvictBM_S: s:slot_id -> s':slot_id -> t:timestamp -> logS_entry
-
+             
 let logS = Seq.seq logS_entry
 
-let drop_slots_aux (e:logSK_entry) :logK_entry =
+let is_state_op (e: logS_entry): bool =
   match e with
-  | Get_SK _ k v -> Spec.Get k v
-  | Put_SK _ k v -> Spec.Put k v
-  | AddM_SK _ r _ k' -> Spec.AddM r k'
-  | EvictM_SK _ k _ k' -> Spec.EvictM k k'
-  | AddB_SK _ r t j -> Spec.AddB r t j
-  | EvictB_SK _ k t -> Spec.EvictB k t
-  | EvictBM_SK _ k _ k' t -> Spec.EvictBM k k' t
-  
-let drop_slots (l:logSK) : logK 
-  = map drop_slots_aux l
+  | Get_S _ _ _ | Put_S _ _ _ -> true
+  | _ -> false
 
-// possibly similar to EAC: check that for every "OP s k ...", k is the last key added at slot s, and has not been evicted 
-let skc (l:logSK) : Type = admit()
+let to_state_op (e:logS_entry {is_state_op e}): Veritas.State.state_op =
+  match e with
+  | Get_S _ k v -> Veritas.State.Get k v
+  | Put_S _ k v -> Veritas.State.Put k v
 
-// add keys in a way that satisfies skc
-let add_consistent_keys (l:logS) : logSK = admit()
+let to_state_op_logS (l: logS) =
+  map to_state_op (filter_refine is_state_op l)
